Prove concatenate_hash_incremental for blake2... Lots of reorganization to do

specs/lemmas/Spec.Hash.Incremental.fst
@@ -5,8 +5,21 @@ module S = FStar.Seq
 open Spec.Agile.Hash
 open Spec.Hash.Definitions
 open Spec.Hash.PadFinish
+open FStar.Mul
+open Lib.IntTypes
 
 #set-options "--max_fuel 0 --max_ifuel 0 --z3rlimit 300"
+
+let update_last_blake (a:hash_alg{is_blake a})
+  (hash:words_state a)
+  (prevlen:nat{prevlen % block_length a = 0})
+  (input:bytes{S.length input + prevlen <= max_input_length a}):
+  Tot (words_state a)
+  = let (nb, rem) = Spec.Blake2.split (to_blake_alg a) (S.length input) in
+    let blocks = Seq.slice input 0 (nb * block_length a) in
+    let (h', totlen) = update_multi a hash blocks in
+    let last_block = Spec.Blake2.get_last_padded_block (to_blake_alg a) input rem in
+    (Spec.Blake2.blake2_update_block (to_blake_alg a) true (v (totlen +. u64 rem)) last_block h', u64 0)
 
 (* An incremental specification better suited to a stateful API, allowing the
    client to perform the padding at the last minute upon hitting the last chunk of
@@ -17,6 +30,9 @@ let update_last (a:hash_alg)
   (input:bytes{S.length input + prevlen <= max_input_length a}):
   Tot (words_state a)
 =
+  if is_blake a then
+    update_last_blake a hash prevlen input
+  else
   let total_len = prevlen + S.length input in
   let padding = pad a total_len in
   update_multi a hash S.(input @| padding)
@@ -26,7 +42,93 @@ let hash_incremental (a:hash_alg) (input:bytes{S.length input <= (max_input_leng
 =
   let open FStar.Mul in
   let n = S.length input / (block_length a) in
+  // Ensuring that we always handle one block in update_last
+  let n = if S.length input % block_length a = 0 && n > 0 then n-1 else n in
   let bs, l = S.split input (n * (block_length a)) in
   let hash = update_multi a (init a) bs in
   let hash = update_last a hash (n * (block_length a)) l in
   finish a hash
+
+let padded_block_modulo (a:hash_alg{is_blake a}) (s1 s2:bytes) (rem:nat{rem <= block_length a}) (n:nat)
+  : Lemma (requires S.length s2 == n * block_length a /\ rem <= S.length s1)
+          (ensures Spec.Blake2.get_last_padded_block (to_blake_alg a) s1 rem `S.equal`
+                   Spec.Blake2.get_last_padded_block (to_blake_alg a) (s2 `S.append` s1) rem)
+  = let last1 = Seq.slice s1 (S.length s1 - rem) (S.length s1) in
+    let s' = s2 `S.append` s1 in
+    let last2 = Seq.slice s' (S.length s' - rem) (S.length s') in
+    assert (Seq.equal last1 last2)
+
+let small_update_last_blake
+  (a:hash_alg{is_blake a}) (h:words_state a)
+  (prevlen:nat{prevlen % block_length a = 0}) (s:bytes)
+  : Lemma
+    (requires S.length s + prevlen <= max_input_length a /\ S.length s <= block_length a)
+    (ensures
+      (let last_block = Spec.Blake2.get_last_padded_block (to_blake_alg a) s (S.length s) in
+      update_last_blake a h prevlen s ==
+      (Spec.Blake2.blake2_update_block (to_blake_alg a) true (v (snd h +. u64 (S.length s))) last_block (fst h), u64 0)))
+   = let (nb, rem) = Spec.Blake2.split (to_blake_alg a) (S.length s) in
+     let blocks = Seq.slice s 0 (nb * block_length a) in
+     let h' = update_multi a h blocks in
+//   TODO: Reorganize modules to avoid circular dependencies
+//     Spec.Hash.Lemmas.update_multi_zero a h
+     assume (h == h')
+
+let blake_split_same_modulo (a:hash_alg{is_blake a}) (len1 len2:nat) (n:nat)
+  : Lemma (requires len1 + n * block_length a = len2 /\ len1 > 0)
+          (ensures snd (Spec.Blake2.split (to_blake_alg a) len1) ==
+                   snd (Spec.Blake2.split (to_blake_alg a) len2))
+  = ()
+
+// TODO: Reorganize modules to avoid circular dependencies
+let update_multi_associative (a: hash_alg)
+  (h: words_state a)
+  (input1: bytes_blocks a)
+  (input2: bytes_blocks a):
+  Lemma (ensures (
+    let input = S.append input1 input2 in
+    (update_multi a (update_multi a h input1) input2) ==
+      (update_multi a h input)))
+  = admit()
+
+#push-options "--z3rlimit 2500"
+
+let concatenated_hash_incremental_blake (a:hash_alg{is_blake a}) (inp1:bytes_blocks a) (inp2:bytes)
+  : Lemma
+    (requires Seq.length (inp1 `S.append` inp2) <= max_input_length a /\ Seq.length inp2 > 0)
+    (ensures finish a (update_last_blake a (update_multi a (init a) inp1) (S.length inp1) inp2)
+      `S.equal` hash_incremental a (inp1 `S.append` inp2))
+  = let open FStar.Mul in
+    let h = init a in
+
+    let h1 = update_multi a h inp1 in
+    let h2 = update_last_blake a h1 (S.length inp1) inp2 in
+    let n = S.length inp2 / (block_length a) in
+    let n:nat = if S.length inp2 % block_length a = 0 && n > 0 then n-1 else n in
+    let nb, rem = Spec.Blake2.split (to_blake_alg a) (S.length inp2) in
+
+    let bs2, l2 = S.split inp2 (n * block_length a) in
+
+    assert (S.length l2 == S.length inp2 - (n * block_length a));
+    let h3 = update_multi a h1 bs2 in
+
+    let input = inp1 `S.append` inp2 in
+    let n' = S.length input / (block_length a) in
+    let n':nat = if S.length input % block_length a = 0 && n' > 0 then n'-1 else n' in
+    blake_split_same_modulo a (S.length inp2) (S.length input) (S.length inp1 / (block_length a));
+    let bs, l = S.split input (n' * (block_length a)) in
+
+    assert (l `S.equal` l2);
+    assert (bs `S.equal` (inp1 `S.append` bs2));
+
+    update_multi_associative a h inp1 bs2;
+    assert (h3 == update_multi a h bs);
+
+    assert (nb == n);
+
+    let h4 = update_last_blake a h3 (S.length inp1 + S.length bs2) l2 in
+
+    let last_block = Spec.Blake2.get_last_padded_block (to_blake_alg a) l2 (S.length l2) in
+    padded_block_modulo a l2 bs2 rem n;
+
+    small_update_last_blake a h3 (S.length inp1 + S.length bs2) l2
