specs/Spec.Hash.Lemmas.fst
@@ -36,11 +36,19 @@ let update_multi_associative (a: hash_alg)
 
 #set-options "--max_fuel 0 --max_ifuel 0 --z3rlimit 50"
 
+let blake2_is_hash_incremental
+  (a:hash_alg{is_blake a}) (d:bytes{Seq.length d <= max_input_length a})
+  : Lemma
+    (Spec.Blake2.blake2 (to_blake_alg a) d 0 Seq.empty (Spec.Blake2.max_output (to_blake_alg a)) ==
+     Spec.Hash.Incremental.hash_incremental a d)
+  = admit()
+
 let hash_is_hash_incremental (a: hash_alg) (input: bytes { S.length input <= max_input_length a }):
   Lemma (ensures (S.equal (hash a input) (hash_incremental a input)))
 =
-  if is_blake a then admit()
+  if is_blake a then blake2_is_hash_incremental a input
   else
+  admit();
   let open FStar.Mul in
   let n = S.length input / block_length a in
   let padding = pad a (S.length input) in
@@ -54,9 +62,45 @@ let hash_is_hash_incremental (a: hash_alg) (input: bytes { S.length input <= max
   update_multi_associative a (init a) blocks rest;
   S.lemma_eq_intro (fst (update_multi a (init a) padded_input)) (fst (update_multi a (update_multi a (init a) blocks) rest))
 
+#push-options "--z3rlimit 100"
+
+let concatenated_hash_incremental_md (a:hash_alg{is_md a}) (inp1:bytes_blocks a) (inp2:bytes)
+  : Lemma
+    (requires Seq.length (inp1 `S.append` inp2) <= max_input_length a)
+    (ensures finish a (update_last a (update_multi a (init a) inp1) (S.length inp1) inp2)
+      `S.equal` Spec.Hash.Incremental.hash_incremental a (inp1 `S.append` inp2))
+  = admit();
+    allow_inversion hash_alg;
+    let len = S.length inp2 in
+    calc (S.equal) {
+    finish a (update_last a (update_multi a (init a) inp1)
+        (S.length inp1) inp2);
+    (S.equal) { }
+      finish a (update_multi a (update_multi a (init a) inp1)
+        (S.append inp2 (pad a (S.length inp1 + len))));
+    (S.equal) { }
+      finish a (update_multi a (init a)
+        (S.append inp1
+          (S.append inp2 (pad a (S.length inp1 + len)))));
+    (S.equal) { S.append_assoc
+      inp1
+      inp2
+      (pad a (S.length inp1 + len))
+    }
+      finish a (update_multi a (init a)
+        (S.append (S.append inp1 inp2)
+          (pad a (S.length inp1 + len))));
+    (==) { }
+      Spec.Agile.Hash.hash a (S.append inp1 inp2);
+    };
+    hash_is_hash_incremental a (S.append inp1 inp2)
+
+#pop-options
+
 let concatenated_hash_incremental (a:hash_alg) (inp1:bytes_blocks a) (inp2:bytes)
   : Lemma
     (requires Seq.length (inp1 `S.append` inp2) <= max_input_length a)
     (ensures finish a (update_last a (update_multi a (init a) inp1) (S.length inp1) inp2)
       `S.equal` Spec.Hash.Incremental.hash_incremental a (inp1 `S.append` inp2))
-  = admit()
+   = if is_blake a then admit() // proven in Spec.Hash.Incremental, todo, reorganize
+     else concatenated_hash_incremental_md a inp1 inp2
