specs/Spec.Hash.Lemmas.fsti
@@ -39,4 +39,4 @@ val concatenated_hash_incremental (a:hash_alg) (inp1:bytes_blocks a) (inp2:bytes
   : Lemma
     (requires Seq.length (inp1 `S.append` inp2) <= max_input_length a)
     (ensures finish a (update_last a (update_multi a (init a) inp1) (S.length inp1) inp2)
-      `S.equal` Spec.Hash.Incremental.hash_incremental a (inp1 `S.append` inp2))
+      `S.equal` hash_incremental a (inp1 `S.append` inp2))
